tests/lean/run/9365.lean
@@ -19,5 +19,4 @@ theorem setZeroHead_spec :
   -- We want to see and name the tuple `t` here in order for us not having to repeat its
   -- definition in t.2.toList.tail below
   rename_i t
-  simp
   exists t.2.toList.tail
