tests/lean/run/spredProofMode.lean
@@ -120,6 +120,44 @@ theorem with_proof (H : A → B) (P Q : SPred σs) : P ⊢ₛ Q → ⌜A⌝ → 
 
 end pureintro
 
+namespace emptyhyp
+
+/--
+trace: σs : List Type
+⊢ ⏎
+  h : ⌜True⌝
+  ⊢ₛ ⌜True⌝
+-/
+#guard_msgs in
+theorem true_named : ⊢ₛ (⌜True⌝ : SPred σs) → ⌜True⌝ := by
+  mintro h
+  trace_state
+  mexact h
+
+/--
+trace: σs : List Type
+⊢ ⏎
+  ⊢ₛ ⌜True⌝
+-/
+#guard_msgs in
+theorem true_unnamed_hidden : ⊢ₛ (⌜True⌝ : SPred σs) → ⌜True⌝ := by
+  mintro _
+  trace_state
+  mpure_intro
+  exact True.intro
+
+theorem or : ⊢ₛ ⌜True⌝ ∨ (⌜False⌝ : SPred σs) := by
+  mpure_intro
+  left
+  exact True.intro
+
+theorem with_proof (H : A → B) (P Q : SPred σs) : P ⊢ₛ Q → ⌜A⌝ → ⌜B⌝ := by
+  mintro _HP _HQ
+  mpure_intro
+  exact H
+
+end emptyhyp
+
 namespace frame
 
 theorem move (P Q : SPred σs) : ⊢ₛ ⌜p⌝ ∧ Q ∧ ⌜q⌝ ∧ ⌜r⌝ ∧ P ∧ ⌜s⌝ ∧ ⌜t⌝ → Q := by
@@ -134,6 +172,12 @@ theorem move_multiple (P Q : SPred σs) : ⊢ₛ ⌜p⌝ ∧ Q ∧ ⌜q⌝ ∧ �
   mcases h with ⟨hp, hQ, hq, rest⟩
   mframe
   mexact hQ
+
+theorem move_all : ⊢ₛ ⌜p⌝ ∧ ⌜q⌝ ∧ ⌜r⌝ ∧ ⌜s⌝ ∧ ⌜t⌝ → (⌜t⌝ : SPred []) := by
+  mintro h
+  mframe
+  mpure_intro
+  grind
 
 end frame
 
